src/dafny/bytecode.dfy
@@ -1334,9 +1334,17 @@ module Bytecode {
             // Calculate available gas
             var gascap := GasCalc.CreateGasCap(st);
             // Apply everything
-            var nst := st.UseGas(gascap).IncNonce().Expand(codeOffset,codeSize).Pop().Pop().Pop().Next();
-            // Pass back continuation
-            State.CREATES(nst.evm,gascap,endowment,code, None)
+            var nst := st.Expand(codeOffset,codeSize).Pop().Pop().Pop().Next();
+            // Sanity check nonce
+            if st.evm.world.Nonce(st.evm.context.address) < MAX_U64
+            then
+                // Charge gas and increment nonce
+                var nnst := nst.UseGas(gascap).IncNonce();
+                // Pass back continuation
+                State.CREATES(nnst.evm,gascap,endowment,code, None)
+            else
+                // Immediate failure (nonce overflow)
+                nst.Push(0)
         else
             State.INVALID(STACK_UNDERFLOW)
     }
@@ -1487,9 +1495,17 @@ module Bytecode {
             // Calculate available gas
             var gascap := GasCalc.CreateGasCap(st);
             // Apply everything
-            var nst := st.UseGas(gascap).IncNonce().Expand(codeOffset,codeSize).Pop().Pop().Pop().Pop().Next();
-            // Pass back continuation
-            State.CREATES(nst.evm,gascap,endowment,code,Some(salt))
+            var nst := st.Expand(codeOffset,codeSize).Pop().Pop().Pop().Pop().Next();
+            // Sanity check nonce
+            if st.evm.world.Nonce(st.evm.context.address) < MAX_U64
+            then
+                // Charge gas and increment nonce
+                var nnst := nst.UseGas(gascap).IncNonce();
+                // Pass back continuation
+                State.CREATES(nnst.evm,gascap,endowment,code,Some(salt))
+            else
+                // Immediate failure (nonce overflow)
+                nst.Push(0)
         else
             State.INVALID(STACK_UNDERFLOW)
     }
